theories/lang_to_mlang/backwards_adequacy.v
@@ -1,0 +1,80 @@
+From Coq Require Import ssreflect.
+From stdpp Require Import strings gmap.
+From transfinite.base_logic.lib Require Export fancy_updates.
+From melocoton.mlanguage Require Import mlanguage.
+From melocoton.mlanguage Require Import weakestpre adequacy.
+From melocoton.lang_to_mlang Require Import lang weakestpre.
+From melocoton.language Require Import language weakestpre.
+From transfinite.base_logic.lib Require Import satisfiable.
+From iris.proofmode Require Import proofmode.
+Import umrel.
+Section BackwardsLiftedAdequacy.
+  Existing Instance ordinals.ordI.
+  Context {val : Type}.
+  Context (Λ : language val).
+  Context {Σ : gFunctors}.
+
+  Context (Φpure : state Λ → val → Prop).
+  Context (p : lang_prog Λ).
+  Context (Ψ : protocol val Σ).
+  Context (Φbi : val → iProp Σ).
+
+  Notation step := (@lang.prim_step _ Λ p).
+  Notation cfg := (prod (expr Λ) (state Λ)).
+
+  Implicit Types σ : state Λ.
+  Implicit Types v : val.
+  Implicit Types e : expr Λ.
+  Implicit Types X : cfg → Prop.
+
+  Definition sideConds `{!invG Σ, !langG val Λ Σ} : iProp Σ := 
+    □ (∀ σ v, state_interp σ ∗ Φbi v ==∗ ⌜Φpure σ v⌝)
+  ∗ □ (∀ f s vv, penv_proto ⟨p,Ψ⟩ f s vv -∗ False).
+  Context `{!invPreG Σ}.
+
+  Context (e : Λ.(expr)).
+  Context (σ : Λ.(state)).
+
+  Context (Halloc : ∀ `{!invG Σ}, Alloc (langG val Λ Σ) (λ H,
+    sideConds ∗ state_interp σ ∗ WP e @ ⟨p,Ψ⟩ ; ⊤ {{Φbi}})%I True).
+
+  Lemma mlang_to_lang_safe e' σ' Φ :
+    @mlanguage.safe _ (lang_to_mlang Λ) p e' σ' Φ → safe p e' σ' Φ.
+  Proof.
+    rewrite /safe /mlanguage.safe /mlanguage.to_val; cbn.
+    destruct (to_val e') eqn:Heq.
+    - done.
+    - intros (X&HX). inversion HX; simplify_eq.
+      by eapply H2.
+  Qed.
+
+  Lemma lang_to_mlang_rtc e1 σ1 e' σ' :
+    rtc_step p e1 σ1 e' σ' → star_AD step (e1, σ1) (λ x, x = (e',σ')).
+  Proof.
+    rewrite /star_AD /= /mrel /=.
+    induction 1.
+    - by eapply star_refl_AD.
+    - eapply star_step_AD. intros Y HY.
+      inversion HY; simplify_eq.
+      exists (e',σ'). split; first by eapply H6.
+      eapply IHrtc_step.
+  Qed.
+
+  Lemma mlang_to_lang_adequacy e' σ':
+    rtc_step p e σ e' σ' → safe p e' σ' (Φpure σ').
+  Proof using All.
+    intros H%lang_to_mlang_rtc.
+    eapply mlang_to_lang_safe.
+    edestruct (@alloc_adequacy_safe _ (lang_to_mlang Λ) _ Φpure p Ψ Φbi _ e σ) as (ex&σx&Heq&HH).
+    - intros HinvG. specialize (Halloc HinvG).
+      intros Φ HT HΦ.
+      destruct (Halloc Φ HT HΦ) as (Hlang&Halloc').
+      exists (lang_to_mlang_mlangG Λ).
+      eapply alloc_mono. 2: exact Halloc'.
+      iIntros "($&($&($&HWP)))".
+      by iApply wp_lang_to_mlang.
+    - exact H.
+    - cbn in Heq. simplify_eq. done.
+  Qed.
+
+End BackwardsLiftedAdequacy.
